\documentclass[12pt,letterpaper,boxed]{hmcpset}

\input{macros}

\usepackage[margin=1in]{geometry}
\usepackage{graphicx}
\usepackage{braket}
\usepackage{bbm}
\usepackage{hyperref}
\usepackage{nameref}
\usepackage{cleveref}

\newcommand{\tukmed}{\hat{\theta}_{\text{Tukey}}}
\newcommand{\geomed}{\hat{\theta}_{\text{geom}}}

\name{Feynman Liang}
\class{EE 290}
\assignment{Problem Set \#1}
\duedate{10/01/2019}

\begin{document}

\begin{problem}[A: Perturbation bound analysis]
	
\end{problem}

\begin{solution}
  \begin{enumerate}
    \item
      \begin{align}
	\|X Y\|_F^2
	= \sum_{i=1}^k \| X y_i \|_2^2
	\leq \|X\|_2 \sum_{i=1}^k \|y_i\|_2^2
	= \|X\|_2 \|Y\|_F^2
      \end{align}
      Apply this to $X = L^{-1}$ and $Y = A = L L^\top$ to find
      \begin{align}
	\| L^{-1} L L^\top \|_F
	= \| L^\top \|_F
	= \| L \|_F
	&\leq \| L^{-1}\|_2 \|A\|_F \\
	\|L^{-1}\|_2^{-1} \|L\|_F
	&\leq \|A\|_F
      \end{align}
      This is the first inequality we wanted to show. 
      For the second, we use the previous identity on $\|A\|_F$
      followed by the original identity on $\|A^{-1}\|_2 \|L\|_F$
      to find
      \begin{align}
	\|A\|_F \|A^{-1}\|_2
	&\geq \|L^{-1}\|_2^{-1} \|L\|_F \|A^{-1}\|_2  \\
	&\geq \|L^{-1}\|_2^{-1} \|A^{-1} L\|_F \\
	&= \|L^{-1}\|_2^{-1} \|(L^{-1})^\top L^{-1} L\|_F
	= \|L^{-1}\|_2^{-1} \|L^{-1}\|_F
      \end{align}

    \item
      Expanding the square, applying triange inequality, and using the original
      inequality
      \begin{align}
	E 
	&= -A + (A + E)
	= L G^\top + G L^\top + G G^\top \\
	\|E\|_F &\leq 2 \|L G^\top\|_F + \|G G^\top\|_F
		\leq 2 \|L\|_2 \|G\|_F + \|G\|_F^2
      \end{align}
      Applyin the quadratic formula to solve in terms of $\|G\|_F$
      and selecting solution by non-negativity gives
      \begin{align}
	\|G\|_F &\geq -\|L\|_2 + \sqrt{\|L\|_2^2 + \|E\|_F} \\
	\frac{\|G\|_F}{\|L\|_2} &\geq \sqrt{1 + \|E\|_F / \|L\|^2_2}  - 1
      \end{align}
      Noting that $\|A\|_2 = \|L L^\top\|_2 \geq \|L\|_2^2$ by
      sub-multiplicativity of spectral norm, we have
      \begin{align}
	\frac{\|G\|_F}{\|L\|_2} 
	&= \frac{\|E\|_F / \|A\|_2}{1 + \sqrt{1 + \|E\|_F / \|A\|_2}}
      \end{align}

      The second inequality with $\kappa(A)$ comes from applying 
      sub-multiplicativity of Frobenius norm instead to get
      \begin{align}
	\|E\|_F &\leq 2 \|L\|_F \|G\|_F + \|G\|_F^2 \\
	\frac{\|G\|_F}{\|L\|_F} &\geq \sqrt{1 + \|E\|_F / \|L\|_F^2}  - 1
      \end{align}
      and noting by the second inequality in problem (1) applied to $\kappa(A)$
      and the first inequality in problem (1)
      \begin{align}
	\kappa(A) \|A\|_F 
	\geq \|L\|_F \|L^{-1}\|_2 \|A\|_F
	\geq \|L\|_F^2  
      \end{align}
  \end{enumerate}
\end{solution}

\begin{problem}[B: Orthogonally invariant norms]
	
\end{problem}

\begin{solution}
	
\end{solution}

\end{document}
